

# **CS-E4830 - Kernel Methods in Machine Learning**

## **Homework Assignment 4 – Pen and Paper**

**Student: Quoc Tuan Vinh, Ngo (704526)**

---

**Question 1. Regularization Requirement in Kernel CCA**

We have the kernel CCA optimization problem as:

$$\begin{aligned} & \max_{\alpha, \beta} \langle K_a \alpha, K_b \beta \rangle \\ & \text{subject to } \|K_a \alpha\|_2 = \sqrt{\alpha^T K_a^2 \alpha} = 1 \text{ and } \|K_b \beta\|_2 = \sqrt{\beta^T K_b^2 \beta} = 1 \end{aligned}$$

Our optimization problem can be reformulated as:

$$\begin{aligned} & \max_{\alpha, \beta} \alpha^T K_a^T K_b \beta \\ & \text{subject to } \alpha^T K_a^2 \alpha = 1 \text{ and } \beta^T K_b^2 \beta = 1 \text{ (can be expressed in squared form)} \end{aligned}$$

Apply Lagrange method, we have:

$$L = \alpha^T K_a^T K_b \beta - \frac{\rho_1}{2} (\alpha^T K_a^2 \alpha - 1) - \frac{\rho_2}{2} (\beta^T K_b^2 \beta - 1) \quad (1)$$

Where  $\rho_1, \rho_2$  are Lagrange multipliers. Taking the derivatives of  $L$  wrt. vectors  $\alpha, \beta$ :

$$\frac{\delta L}{\delta \alpha} = K_a K_b \beta - \rho_1 K_a^2 \alpha \quad (2)$$

$$\frac{\delta L}{\delta \beta} = K_b K_a \alpha - \rho_2 K_b^2 \beta \quad (3)$$

Setting both (2) and (3) to zero, and multiplying (2) from the left by  $\alpha^T$  and (3) from the left by  $\beta^T$ , we have:

$$\alpha^T K_a K_b \beta - \rho_1 \alpha^T K_a^2 \alpha = 0 \quad (4)$$

$$\beta^T K_b K_a \alpha - \rho_2 \beta^T K_b^2 \beta = 0 \Leftrightarrow \alpha^T K_a K_b \beta - \rho_2 \beta^T K_b^2 \beta = 0 \quad (5)$$

Since  $\alpha^T K_a^2 \alpha = 1$  and  $\beta^T K_b^2 \beta = 1$ , from (4) and (5), we get that  $\rho_1 = \rho_2 = \rho$ . Therefore, from (2), we have:

$$K_a K_b \beta - \rho_1 K_a^2 \alpha = K_a K_b \beta - \rho K_a^2 \alpha = 0 \Leftrightarrow \alpha = \frac{1}{\rho} K_a^{-1} K_a^{-1} K_a K_b \beta = \frac{1}{\rho} K_a^{-1} K_b \beta \quad (6)$$

Substitute (6) into (3), we obtain:

$$\begin{aligned} K_b K_a \alpha - \rho_2 K_b^2 \beta &= \frac{1}{\rho} K_b K_a K_a^{-1} K_b \beta - \rho K_b^2 \beta = \frac{1}{\rho} K_b^2 \beta - \rho K_b^2 \beta = 0 \\ \Leftrightarrow K_b^2 \beta &= \rho^2 K_b^2 \beta \Leftrightarrow I \beta = \rho^2 \beta \quad (7) \end{aligned}$$

One problem when obtaining (6) and (7) is that kernels  $K_a, K_b$  must be invertible. To guarantee this, we can regularize these two by adding a regularized constant  $c_1, c_2$  respectively to the diagonal of kernel  $K_a, K_b$ . Therefore, our restrictions now become:

$$\alpha^T (K_a + c_1 I)^2 \alpha = 1 \text{ and } \beta^T (K_b + c_2 I)^2 \beta = 1 \quad (8)$$

The solutions then can be found by solving the standard eigenvalue problem:

$$(K_b + c_2 I)^{-2} K_b K_a (K_a + c_1 I)^{-2} K_a K_b \alpha = \rho^2 \alpha \quad (9)$$

Similarly to CCA case, the formulation can be explained as:

$$\begin{pmatrix} 0 & K_a K_b \\ K_b K_a & 0 \end{pmatrix} \begin{pmatrix} \alpha \\ \beta \end{pmatrix} = \rho \begin{pmatrix} (K_a + c_1 I)^2 & 0 \\ 0 & (K_b + c_2 I)^2 \end{pmatrix} \begin{pmatrix} \alpha \\ \beta \end{pmatrix}$$

**Question 2.** *Kernel CCA is CCA on Hilbert Space Objects*

We need to prove:

$$\widehat{cov}(\langle \phi_a(x_a), w_a \rangle, \langle \phi_b(x_b), w_b \rangle) = \frac{1}{n} \alpha^T K_a^T K_b \beta$$

Let  $S_a$  and  $S_b$  represent the linear spaces spanned by the images of the data points. For any  $w_a \in \mathcal{H}_a, w_b \in \mathcal{H}_b$ , we have  $w_a = w_a^{\parallel} + w_a^{\perp}$ , where  $w_a^{\parallel} = \sum_{k=1}^n \alpha_k \phi_a(x_a^k) \in S_a$  and  $w_a^{\perp}$  is orthogonal to all objects  $\phi_a \in S_a$ . The same logic applies to  $w_b$ .

Therefore, we can derive the empirical covariance of the transformations in the feature space as below:

$$\begin{aligned} \widehat{cov}(\langle \phi_a(x_a), w_a \rangle, \langle \phi_b(x_b), w_b \rangle) &= \frac{1}{n} \sum_{k=1}^n \langle \phi_a(x_a^k), w_a \rangle \langle \phi_b(x_b^k), w_b \rangle \\ &= \frac{1}{n} \sum_{k=1}^n \langle \phi_a(x_a^k), w_a^{\parallel} + w_a^{\perp} \rangle \langle \phi_b(x_b^k), w_b^{\parallel} + w_b^{\perp} \rangle \\ &= \frac{1}{n} \sum_{k=1}^n (\langle \phi_a(x_a^k), w_a^{\parallel} \rangle + \langle \phi_a(x_a^k), w_a^{\perp} \rangle) (\langle \phi_b(x_b^k), w_b^{\parallel} \rangle + \langle \phi_b(x_b^k), w_b^{\perp} \rangle) \quad (1) \end{aligned}$$

Since  $\langle \phi_a(x_a^k), w_a^{\perp} \rangle = \langle \phi_b(x_b^k), w_b^{\perp} \rangle = 0$ , (1) can be simplified as:

$$\begin{aligned} (1) &= \frac{1}{n} \sum_{k=1}^n (\langle \phi_a(x_a^k), w_a^{\parallel} \rangle) (\langle \phi_b(x_b^k), w_b^{\parallel} \rangle) \\ &= \frac{1}{n} \sum_{k=1}^n \langle \phi_a(x_a^k), \sum_{i=1}^n \alpha_i \phi_a(x_a^i) \rangle \langle \phi_b(x_b^k), \sum_{j=1}^n \beta_j \phi_b(x_b^j) \rangle \\ &= \frac{1}{n} \sum_{k=1}^n \sum_{i=1}^n \sum_{j=1}^n \alpha_i \langle \phi_a(x_a^i), \phi_a(x_a^k) \rangle \langle \phi_b(x_b^j), \phi_b(x_b^k) \rangle \beta_j \\ &= \frac{1}{n} \sum_{k=1}^n \sum_{i=1}^n \sum_{j=1}^n \alpha_i K_a(x_a^i, x_a^k) K_b(x_b^j, x_b^k) \beta_j = \frac{1}{n} \alpha^T K_a^T K_b \beta \end{aligned}$$

Which is what we need to prove.